Update quantum_hoare_logic.thy

quantum_hoare_logic.thy
@@ -2,6 +2,7 @@ theory quantum_hoare_logic
 imports Main  basic
 begin
 
+(*The datatype for representing syntax of quantum programs*)
 datatype
 com=SKIP
 |Init "nat list" "number"
@@ -11,6 +12,19 @@ com=SKIP
 |While "Mat" "Mat" "com" "Mat" 
 |While_n "Mat" "Mat" "com" "Mat" "nat"
 
+primrec M_sum::"(Mat*com*Mat) list\<Rightarrow>Mat"where
+"M_sum [] =I"|
+"M_sum (a#M) =mat_add (mat_mult (dag (fst a) ) (fst a)) (M_sum M )"
+(*the conditions the comands should meet they are well-defined  *)
+primrec wellDefined :: "com\<Rightarrow>bool" where
+"wellDefined SKIP =True"|
+"wellDefined (Utrans a n) = (a \<in> uMat)"|
+"wellDefined (Init m n) =True"|
+"wellDefined (s1;s2) = (wellDefined (s1) & wellDefined (s2))"|
+"wellDefined (Cond mcl) = (M_sum mcl=I) "|
+"wellDefined (While_n m0 m1 s Q n)= (mat_add (mat_mult (dag m0) m0)  (mat_mult (dag m1) m1) =I)" |
+"wellDefined  (While  m0 m1 s Q )=(mat_add (mat_mult (dag m0) m0)  (mat_mult (dag m1) m1) =I)  "
+
 primrec sum::"nat list\<Rightarrow>nT\<Rightarrow>Mat\<Rightarrow>nT\<Rightarrow>Mat" where
 "sum [] f1 p g1=zero"|
 "sum (b#nl) f1 p g1 = mat_add (mat_mult (mat_mult (f1 b) p) (g1 b)) (sum nl f1 p g1)"
@@ -19,7 +33,6 @@ primrec sum_1::"nat list\<Rightarrow>nT\<Rightarrow>nT\<Rightarrow>Mat" where
 "sum_1 [] f1 g1=zero"|
 "sum_1 (b#nl) f1 g1=mat_add (mat_mult (f1 b) (g1 b)) (sum_1 nl f1 g1)"
 (*  f(1)*g(1)+f(2)*g(2)+..\<doteq>I the same as measurement matrix      *)
-
 axiomatization where
 fg:"sum_1 m g f=I"
 
@@ -29,7 +42,7 @@ definition u::"Mat\<Rightarrow>Mat\<Rightarrow>Mat"where
 (*u a b =(dag a)ba *)
 definition uu::"Mat\<Rightarrow>Mat\<Rightarrow>Mat"where
 "uu a b= mat_mult (mat_mult (dag a) b)  a"
- 
+ (*the rank that defined for the command*)
 fun rank :: "com\<Rightarrow>nat" where
 "rank SKIP =1"|
 "rank (Utrans U n) =1"|
@@ -43,12 +56,13 @@ fun rank :: "com\<Rightarrow>nat" where
 lemma rank_pos : " rank ss > 0" 
 apply (induct ss, auto) 
 by (smt2 One_nat_def Suc_less_eq le_imp_less_Suc list.case(1) list.case(2) list.exhaust monoid_add_class.add.left_neutral monoid_add_class.add.right_neutral not_le order_refl plus_nat.simps(2) rank.simps(5) trans_le_add1 trans_le_add2)
-
+(*definition of fixpoint*)
 definition fixpoint::"Mat\<Rightarrow>Mat\<Rightarrow>com\<Rightarrow>Mat\<Rightarrow>Mat\<Rightarrow>Mat"where
 "fixpoint m0 m1 s Q p=fixPoint"
 definition fixpoint_wlp::"Mat\<Rightarrow>Mat\<Rightarrow>com\<Rightarrow>Mat\<Rightarrow>Mat\<Rightarrow>Mat"where
 "fixpoint_wlp  m0 m1 s Q p=fixPoint_wlp"
 
+(*the denotational semantics of quantum programs  *)
 function denoFun::"com\<Rightarrow>Mat\<Rightarrow>Mat" where
 "denoFun SKIP p=p"|
 "denoFun (Utrans U n) p=mat_mult (mat_mult U p) (dag U)"|
@@ -64,27 +78,24 @@ by  pat_completeness auto
 termination 
  apply (relation "measure (\<lambda>(c,m).rank c)", auto )
 by (metis rank_pos)
-
+(*the ascending  order of denotational semantics of while_n *)
 lemma ascend:"\<forall> \<rho> .less  (denoFun (While_n m0 m1 s Q n) \<rho>)   (denoFun (While_n m0 m1 s Q (Suc n) ) \<rho>)"
 apply(induct n,auto)
-apply(simp add:zero_rel)
-apply(rule less1)
-apply auto
-done
+apply (metis (poly_guards_query) Ident zero_mult_l I_zero fg sum_1.simps(1))
+by (metis Nitpick.case_nat_unfold less1)
 
+(*the definition of valid *)
 definition valid::"Mat\<Rightarrow>com\<Rightarrow>Mat\<Rightarrow>bool" where
-"  valid P S Q= (\<forall>\<rho>.  Tr (mat_mult P \<rho>)<= Tr (mat_mult Q (denoFun S \<rho>))+Tr \<rho>-Tr (denoFun S \<rho>)   )"
-
+"  valid P S Q= (\<forall>\<rho>. \<rho> \<in> rhoMat\<longrightarrow> Tr (mat_mult P \<rho>)<= Tr (mat_mult Q (denoFun S \<rho>))+Tr \<rho>-Tr (denoFun S \<rho>)   )"
+(*svalid is equal to valid ,just for simplication*)
 definition svalid::"Mat\<Rightarrow>com\<Rightarrow>Mat\<Rightarrow>bool"where
-"svalid P S Q=(\<forall> \<rho>. Tr (mat_mult (mat_sub I Q) (denoFun S \<rho>)) <= Tr (mat_mult (mat_sub I P) \<rho>) )"
+"svalid P S Q=(\<forall> \<rho> .\<rho>\<in>rhoMat\<longrightarrow> Tr (mat_mult (mat_sub I Q) (denoFun S \<rho>)) <= Tr (mat_mult (mat_sub I P) \<rho>) )"
 lemma eq_valid:"svalid P S Q  \<Longrightarrow>valid P S Q"
 apply(simp add:valid_def)
 apply(simp add:svalid_def)
 apply(simp add:mult_sub_allo1)
 apply(simp add:tr_allo1)
-apply(simp add:I_mult)
-apply auto
-apply(drule_tac x=" \<rho>" in spec) 
+apply(simp add:Ident)
 apply auto
 done
 lemma eq_valid2:"valid P S Q\<Longrightarrow>svalid P S Q"
@@ -92,16 +103,14 @@ apply(simp add:valid_def)
 apply(simp add:svalid_def)
 apply(simp add:mult_sub_allo1)
 apply(simp add:tr_allo1)
-apply(simp add:I_mult)
-apply auto
-apply(drule_tac x=" \<rho>" in spec) 
+apply(simp add:Ident)
 apply auto
 done
 lemma b1:" (mat_mult (mat_mult (mat_mult a b) c) d) =mat_mult (mat_mult a b) (mat_mult c d)"
-apply (simp add:mult_asso)
+apply (simp add:mult_exchange)
 done
 lemma b2:" (mat_mult (mat_mult b d) (mat_mult a c)) =mat_mult (mat_mult (mat_mult b d) a) c"
-apply (simp add:mult_asso)
+apply (simp add:mult_exchange)
 done
 lemma b3:" Tr (mat_mult (mat_mult (mat_mult e  b) d) c)=Tr (mat_mult b (mat_mult (mat_mult d c) e ))"
 apply(simp add:b1)
@@ -110,7 +119,7 @@ apply(simp add:b2)
 apply(simp add:exchange)
 done
 lemma b4:"mat_mult (dag U) (mat_mult U \<rho>) =mat_mult(mat_mult (dag U) U) \<rho>"
-apply(simp add:mult_asso)
+apply(simp add:mult_exchange)
 done
 
 lemma hh:" Tr (mat_mult (f a) (mat_mult \<rho> (g a))) =Tr (mat_mult (mat_mult \<rho> (g a))   (f a))"
@@ -119,18 +128,18 @@ done
 lemma temp:"Tr (sum m f \<rho> g) =Tr  (mat_mult \<rho> (sum_1 m g f) ) "
 apply(induct m)
 apply auto
-apply(simp add:zero_mult)
-apply(simp add:mult_dist_l)
+apply(simp add:zero_mult_r)
+apply(simp add:mult_allo2)
 apply(simp add:tr_allo)
-apply(simp add:mult_asso)
+apply(simp add:mult_exchange)
 apply(simp add:hh)
-apply(simp add:mult_asso)
+apply(simp add:mult_exchange)
 done
 lemma m_init:"Tr (sum m f \<rho> g) =Tr \<rho>"
 apply(simp add:temp)
 apply(simp add:fg)
 apply(subgoal_tac " Tr (mat_mult \<rho> I) = Tr (mat_mult I \<rho> ) ")
-apply(simp add:I_mult)
+apply(simp add:Ident)
 apply(simp add:exchange)
 done
 
@@ -142,7 +151,8 @@ svalid Q S  (mat_add (uu m0 P) (uu m1 Q)) ; svalid Q S  (mat_add (uu m0 P) (uu m
         \<le> Tr (mat_mult (mat_sub I (mat_add (uu m0 P) (uu m1 Q))) \<rho>) )"
 apply auto
 done
-lemma While_n:"mat_add  (mat_mult m0 (dag m0)) (mat_mult m1 (dag m1)) =I\<Longrightarrow>
+
+lemma While_n:"wellDefined (While_n m0 m1 S Q n) \<Longrightarrow>mat_add  (mat_mult m0 (dag m0)) (mat_mult m1 (dag m1)) =I\<Longrightarrow>
 valid Q S (mat_add (uu m0 P) (uu m1 Q)) \<Longrightarrow> 
 \<forall>\<rho>. Tr (mat_mult (mat_sub I P)  (denoFun (While_n m0 m1 S Q n) \<rho>))
         \<le> Tr (mat_mult (mat_sub I (mat_add (uu m0 P) (uu m1 Q))) \<rho>) "
@@ -151,12 +161,11 @@ apply(simp add:eq_valid2)
 prefer 2
 apply auto
 apply(induct n)
-apply(simp add:zero_mult)
+apply(simp add:zero_mult_r)
 apply(simp add:zero_tr)
-apply(simp add:\<rho>_rel)
 apply(simp add:svalid_def)
-apply(split nat.split)
-by (metis (mono_tags, hide_lams) I_mult U_dag zero_mult zero_mult_l)
+apply (metis (poly_guards_query) Ident zero_mult_l zero_tr fg less_irrefl not_le sum_1.simps(1))
+by (metis (full_types) Ident zero_mult_r zero_mult_l zero_tr denoFun.simps(6) exchange fg monoid_add_class.add.right_neutral mult_exchange mult_sub_allo1 order_refl sum_1.simps(1) tr_allo u_def uu_def)
 primrec sum1::"(Mat*com*Mat) list\<Rightarrow>Mat"where
 "sum1 []  =zero"|
 "sum1  (a#M)  =  (mat_add (uu (fst a ) (snd (snd a)))  (sum1 M  ))  "
@@ -184,23 +193,23 @@ done
 lemma Skip:"valid P SKIP P"
 apply (simp add:valid_def)
 done
-lemma Utrans:"valid  (mat_mult (mat_mult (dag U) P) U)  (Utrans U n) P"
+lemma Utrans:"wellDefined (Utrans U n) \<Longrightarrow>valid  (mat_mult (mat_mult (dag U) P) U)  (Utrans U n) P"
 apply(simp add:valid_def)  
 apply(simp add:b3)
 apply(simp add:exchange)
 apply(simp add:b4)
 apply(simp add:U_dag)
-apply(simp add:I_mult)
+apply(simp add:Ident)
 done
 lemma Init:"valid (sum m g P f)  (Init m n) P"
 apply(simp add:valid_def, auto)
 apply(simp add:m_init)
 apply (induct m)
 apply (simp add:valid_def, auto)
-apply(simp  add:zero_mult)
+apply(simp  add:zero_mult_r)
 apply(simp add:zero_mult_l)
-apply(simp add:mult_dist)
-apply(simp add:mult_dist_l)
+apply(simp add:mult_allo1)
+apply(simp add:mult_allo2)
 apply(simp add:tr_allo)
 apply(simp add:b3)
 done
@@ -209,17 +218,17 @@ apply(simp add:valid_def,auto)
 apply(drule_tac x=" \<rho>" in spec)
 apply(drule_tac x="denoFun s1 \<rho>" in spec)
 apply auto
-done
+by (metis (full_types) Ident zero_mult_l fg sum_1.simps(1))
 
-lemma Measure:"validlist M Q \<Longrightarrow>   valid (sum1 M) (Cond M ) Q" 
+lemma Measure:"wellDefined (Cond M) \<Longrightarrow>validlist M Q \<Longrightarrow> valid (sum1 M) (Cond M ) Q" 
 apply (induct M)
 apply(simp add:valid_def,auto)
-apply(simp add:zero_mult)
+apply(simp add:zero_mult_r)
 apply(simp add:zero_mult_l)
 apply(simp add:zero_tr)
-apply(simp add:\<rho>_rel)
+apply(simp add:c)
 apply(simp add:valid_def uu_def,auto)
-by (smt2 I_mult zero_mult_l zero_tr fg sum_1.simps(1))
+by (smt2 Ident zero_mult_l zero_tr fg sum_1.simps(1))
 
 (* fixpoint theory  *)
 axiomatization where
@@ -228,7 +237,7 @@ axiomatization where
                 Tr (mat_mult p (fixpoint  m0 m1 s Q \<rho>) )\<le>x"
 
 
-lemma While:"valid Q S (mat_add (uu m0 P) (uu m1 Q)) \<Longrightarrow>valid (mat_add (uu m0 P) (uu m1 Q)) 
+lemma While:"wellDefined (While m0 m1 S Q) \<Longrightarrow>valid Q S (mat_add (uu m0 P) (uu m1 Q)) \<Longrightarrow>valid (mat_add (uu m0 P) (uu m1 Q)) 
           (While m0 m1 S Q ) P"
 apply(rule eq_valid)
 apply(rule w4,auto)
@@ -238,8 +247,8 @@ unfolding svalid_def
 apply auto
 apply(rule fixpoint_lemma,auto)
 prefer 2
-apply (metis (full_types) I_mult U_dag zero_mult zero_mult_l \<rho>_rel zero_tr denoFun.simps(6) exchange mult_asso mult_sub_allo1 u_def uu_def)
-by (metis (mono_tags, lifting) I_mult U_dag zero_mult_l zero_rel mult_asso)
+apply (metis (full_types) Ident zero_mult_l zero_tr denoFun.simps(6) exchange fg less_irrefl mult_exchange not_le sum_1.simps(1) u_def uu_def)
+by (metis (mono_tags) Ident zero_mult_l rho_zero fg sum_1.simps(1))
 
 lemma order:"\<lbrakk>less P Pa;valid Pa S Q\<rbrakk>\<Longrightarrow>valid P S Q"
 apply(simp add:valid_def)
@@ -252,7 +261,8 @@ lemma Order:"\<lbrakk>less P Pa;valid Pa S Qa;less Qa Q\<rbrakk>\<Longrightarrow
 apply(simp add:valid_def,auto)
 apply(drule_tac x=" \<rho>" in spec)
 apply(rule o1,auto)
-by (metis (full_types) I_mult U_dag zero_mult ab_left_minus add.commute add_uminus_conv_diff zero_mult_l zero_tr monoid_add_class.add.left_neutral order_refl tr_allo tr_allo1)
+by (metis (poly_guards_query) Ident zero_mult_l fg sum_1.simps(1))
+
 
 (*     about wlp          *)
 definition matsum::"nat list\<Rightarrow>nat\<Rightarrow>Mat\<Rightarrow>Mat" where
@@ -278,8 +288,9 @@ by (metis rank_pos)
 
 lemma ascent_wlp:"less (wlp P (While_n m0 m1 s Q n))  (wlp P (While_n m0 m1 s Q (Suc n)))"
 apply(induct n,auto)
-apply (metis U_dag zero_mult zero_rel)
-by (metis (mono_tags, lifting) I_mult U_dag zero_mult_l mult_asso)
+apply (metis (poly_guards_query) Ident zero_mult_l I_zero fg sum_1.simps(1))
+by (metis (mono_tags) Ident zero_mult_l fg sum_1.simps(1))
+
 axiomatization where
  fixpoint_wlp_lemma:"\<forall> n .less (wlp P (While_n m0 m1 s Q n))  (wlp P (While_n m0 m1 s Q (Suc n)))\<Longrightarrow>
                  \<forall> n. Tr (mat_mult  (wlp P (While_n m0 m1 s Q n)) p ) \<le> x\<Longrightarrow>
@@ -294,30 +305,32 @@ apply(simp add:matsum_def)
 apply(simp add:Init)
 done
 (*    Utrans        *)
-lemma wlp_utrans: "valid (wlp P (Utrans U n)) (Utrans U n) P"
+lemma wlp_utrans: "wellDefined (Utrans U n) \<Longrightarrow>valid (wlp P (Utrans U n)) (Utrans U n) P"
 apply(simp add:matUtrans_def)
 apply(simp add:Utrans)
 done
 (*     Cond Measure       *)
-lemma wlp_cond: "valid (wlp Q (Cond M )) (Cond M )  Q"
+lemma wlp_cond: " wellDefined (Cond M) \<Longrightarrow> valid (wlp Q (Cond M )) (Cond M )  Q"
 apply(simp add:valid_def uu_def)
-by (metis (no_types, lifting) I_mult U_dag zero_mult exchange less_irrefl not_le tr_allo tr_allo1)
+by (metis (mono_tags, lifting) Ident zero_mult_l fg less_irrefl not_le sum_1.simps(1) tr_allo tr_allo1)
 (*  While_n     *)
-lemma wlp_while_n:" \<forall>Q. valid (wlp Q com) com Q \<Longrightarrow>
+lemma wlp_while_n:"Q\<in>predMat\<Longrightarrow> wellDefined (While_n Mata Matb com Matc m) \<Longrightarrow> \<forall>Q. valid (wlp Q com) com Q \<Longrightarrow>
        valid (case num of 0 \<Rightarrow> I | Suc m \<Rightarrow> mat_add (uu Mata Q) (uu Matb (wlp (wlp Q (While_n Mata Matb com Matc m)) com))) (While_n Mata Matb com Matc num) Q"
 apply(split nat.split,auto)
 apply(simp add:valid_def,auto)
-apply(simp add:I_mult)
-apply (metis zero_mult zero_tr diff_0_right order_refl)
+apply(simp add:Ident)
+apply (metis zero_mult_r zero_tr diff_0_right order_refl)
 apply(simp add:valid_def,auto)
-by (metis I_mult U_dag zero_mult exchange linordered_field_class.sign_simps(16))
+by (metis (mono_tags, lifting) Ident zero_mult_l fg sum_1.simps(1) u_def)
+
 (*While   *)
-lemma wlp_while:"\<forall>Q. valid (wlp Q com) com Q \<Longrightarrow>
+lemma wlp_while:" wellDefined (While Mata Matb com Matc ) \<Longrightarrow>\<forall>Q. valid (wlp Q com) com Q \<Longrightarrow>
        valid (fixpoint_wlp Mata Matb com Matc Q)  (While Mata Matb com Matc ) Q"
 apply(simp add:valid_def,auto)
 apply(rule fixpoint_wlp_lemma,auto)
-apply (metis (mono_tags, lifting) I_mult U_dag zero_mult zero_rel mult_asso)
-by (metis I_mult U_dag zero_mult exchange)
+apply (smt2 Ident ascend zero_mult_l fg sum_1.simps(1))
+by (metis (full_types) Ident zero_mult_l fg sum_1.simps(1))
+
 (*    Seq     *)
 lemma wlp_seq: "\<forall>Q. valid (wlp Q coma) coma Q \<Longrightarrow> \<forall>Q. valid (wlp Q comb) comb Q 
    \<Longrightarrow> valid (wlp (wlp Q comb) coma) (coma; comb) Q"
@@ -325,23 +338,25 @@ apply (drule_tac x = "(wlp Q comb)" in  spec)
 apply (drule_tac x = "Q" in  spec)
 apply (rule Seq, auto)
 done
-lemma soundwp1: "\<forall> Q. valid (wlp Q S) S  Q"
-apply (induct_tac S, auto)
+lemma soundwp1: "wellDefined S \<Longrightarrow>\<forall> Q. valid (wlp Q S) S  Q"
+apply (induct S,auto)
 apply (cut_tac wlp_skip, auto)
 apply (cut_tac wlp_init, auto)
 apply (cut_tac wlp_utrans, auto)
-apply (cut_tac Q = Q and  coma = "com1" and comb = "com2" in wlp_seq, auto)
+apply (cut_tac Q = Q and  coma = "S1" and comb = "S2" in wlp_seq, auto)
 apply (cut_tac wlp_cond, auto)
 defer
-apply(cut_tac wlp_while_n,auto)
-apply(cut_tac Mata="Mat1" and Matb="Mat2" and Matc="Mat3" and com="com" and Q="Q" in wlp_while,auto)
-done
-lemma WLPsound:"valid (wlp Q S) S Q"
+apply (metis (poly_guards_query) Ident zero_mult_l eq_valid fg less_irrefl not_le sum_1.simps(1) svalid_def)
+apply(cut_tac Mata="Mat1" and Matb="Mat2" and Matc="Mat3" and com="S" and Q="Q" in wlp_while,auto)
+by (metis (poly_guards_query) Ident zero_mult_l fg order_refl sum_1.simps(1) tr_allo tr_allo1 valid_def)
+
+lemma WLPsound:"Q\<in>predMat\<Longrightarrow>wellDefined S\<Longrightarrow>valid (wlp Q S) S Q"
 apply(simp add: soundwp1)
 done
-lemma ord_wlp:"less P (wlp Q S)\<Longrightarrow>valid P S Q"
+lemma ord_wlp:"Q\<in>predMat\<Longrightarrow>P\<in>predMat\<Longrightarrow>wellDefined S\<Longrightarrow>less P (wlp Q S)\<Longrightarrow>valid P S Q"
 apply(rule_tac Pa="wlp Q S" in order,auto)
 apply(rule WLPsound)
+apply auto
 done
 declare uu_def[simp]
 ML_file "Quantum_Hoare_tac.ML"
